tests/lean/Hashmap/Properties.lean
@@ -316,10 +316,10 @@ theorem insert_in_list_spec {α : Type} (l : Nat) (key: Usize) (value: α) (l0: 
 -- Remark: α and β must live in the same universe, otherwise the
 -- bind doesn't work
 theorem if_update_eq
-  {α β : Type u} (b : Bool) (y : α) (e : Result α) (f : α → Result β) :
-  (if b then Bind.bind e f else f y) = Bind.bind (if b then e else pure y) f
+  {α : Type u} {β : Type v} (b : Bool) (y : α) (e : Result α) (f : α → Result β) :
+  (if b then Std.bind e f else f y) = Std.bind (if b then e else ok y) f
   := by
-  split <;> simp [Pure.pure]
+  split <;> simp
 
 def frame_slots_params (hm1 hm2 : HashMap α) :=
   -- The max load factor is the same
